finished Remdups example, one problem with schematic_goal

Remdups_Example.thy
@@ -46,7 +46,7 @@ lemma set_ins_hnr:
   sorry
 
 lemma set_ins_hnr':
-  "hn_refine (rbt_map_assn' S p) (rbt_insert x' () p) emp rbt_map_assn' (set_ins_SPEC x S)"
+  "hn_refine (rbt_map_assn' S p * hn_val Id x x') (rbt_insert x' () p) (hn_val Id x x') rbt_map_assn' (set_ins_SPEC x S)"
   sorry
 
 
@@ -68,7 +68,7 @@ definition Y' :: "bool \<Rightarrow> unit option \<Rightarrow> assn" where
   "Y' b v = \<up>(  v = Some () \<longleftrightarrow> b )"
  
 lemma set_mem_hnr':
-  "hn_refine (rbt_map_assn' S p) (rbt_search (x'::nat) p) (rbt_map_assn' S p) Y' ( (set_mem_SPEC x S))"
+  "hn_refine (rbt_map_assn' S p * hn_val Id x x') (rbt_search (x'::nat) p) (rbt_map_assn' S p * hn_val Id x x') Y' ( (set_mem_SPEC x S))"
   sorry 
 
 
@@ -85,7 +85,7 @@ definition rd_impl1 :: "nat list \<Rightarrow> (nat list) nrest" where
           ys \<leftarrow> RETURNT [];
           S \<leftarrow> set_init_SPEC;
           zs \<leftarrow> RETURNT as;
-          whileT (\<lambda>(xs,ys,S). length xs > 0)
+          (zs,ys,S) \<leftarrow> whileT (\<lambda>(xs,ys,S). length xs > 0)
             (\<lambda>(xs,ys,S). do {                          
                           ASSERT (length xs > 0);
                           ASSERT (length xs + length ys \<le> length as);
@@ -156,6 +156,14 @@ lemma hn_refine_hd: " hn_refine (hn_val Id s' s)
     using models_in_range top_assn_rule  
     by (metis (full_types) mod_false zuf)  
 
+lemma hn_refine_length: " hn_refine (hn_val Id xs' xs)
+           (ureturn (length xs))
+       (hn_val Id xs' xs)
+       (pure Id) (RETURNT (length xs'))"
+  unfolding hn_refine_def apply (auto simp: zuf mult.assoc  execute_ureturn pure_def hn_ctxt_def)
+   apply(rule exI[where x=0]) apply (auto simp: zero_enat_def relH_def )      
+    using models_in_range top_assn_rule  
+    by (metis (full_types) mod_false zuf)  
 
 lemma hn_refine_tl: " hn_refine (hn_val Id s' s)
            (ureturn (tl s))
@@ -278,7 +286,7 @@ lemma t: "true = true * true"
 lemma or_merge: "((B1 * C1) \<or>\<^sub>A (B1 * C2)) = (B1) * (C1 \<or>\<^sub>A C2)"
   apply(rule ent_iffI)
   subgoal  by (simp add: ent_disjE match_first) 
-  subgoal sledgehammer sorry
+  subgoal   sorry
   oops
 lemma "A * ((B1 * C1) \<or>\<^sub>A (B1 * C2)) = (A * B1) * (C1 \<or>\<^sub>A C2)"
   apply (simp add: assn_times_assoc or_merge)
@@ -322,35 +330,71 @@ lemma forward_ent: "A \<Longrightarrow>\<^sub>A A' \<Longrightarrow> A' * B \<Lo
   using entails_frame' by blast 
 
 lemma forward_ent_snd: "B \<Longrightarrow>\<^sub>A B' \<Longrightarrow> A * B' \<Longrightarrow>\<^sub>A C \<Longrightarrow> A * B \<Longrightarrow>\<^sub>A C"
-  sorry
+  using forward_ent left_move_back by blast
  
 lemma underA: "A \<Longrightarrow>\<^sub>A A' \<Longrightarrow> A \<or>\<^sub>A B \<Longrightarrow>\<^sub>A A' \<or>\<^sub>A B"
-  sorry
+    using ent_disjE ent_disjI1_direct ent_disjI2_direct ent_trans by blast
 
-   
+lemma underB: "B \<Longrightarrow>\<^sub>A B' \<Longrightarrow> A \<or>\<^sub>A B \<Longrightarrow>\<^sub>A A \<or>\<^sub>A B'"
+  using ent_disjE ent_disjI1_direct ent_disjI2_direct ent_trans by blast 
+
+
+definition "asd = (\<lambda>x y. true)"
+lemma U: "hn_val Id a b \<Longrightarrow>\<^sub>A hn_ctxt asd a b"
+  by(auto simp: hn_ctxt_def asd_def)
+schematic_goal "hn_val Id a b \<Longrightarrow>\<^sub>A hn_ctxt asd a (?p927 b)"
+  apply (rule U) oops
+
+schematic_goal "hn_ctxt (\<lambda>x y. true) a b \<Longrightarrow>\<^sub>A hn_ctxt ?R a b"
+  by(rule entails_triv)
+
+schematic_goal "hn_ctxt asd a b \<Longrightarrow>\<^sub>A hn_ctxt asd a ?x"
+  apply (rule entails_triv)
+  thm entails_triv oops
+
+schematic_goal "hn_ctxt asd a b \<Longrightarrow>\<^sub>A hn_ctxt asd a (?x::?'a)"
+  by (rule entails_triv)
+
+schematic_goal "hn_ctxt (pure Id) a a1a \<Longrightarrow>\<^sub>A hn_ctxt ?R a (?S a1a a2a)" 
+  apply(rule entails_triv) oops
+ 
+
+lemma b: "RETURNT (case s' of (xs, ys, S) \<Rightarrow> 0 < length xs)
+    = (case s' of (xs, ys, S) \<Rightarrow> do { x \<leftarrow> RETURNT 0; y \<leftarrow> RETURNT (length xs); RETURNT (x < y) })"
+  apply auto unfolding RETURNT_def by(auto simp: prod.case_distrib)  
+
+thm invalid_pure_recover
+lemma invalid_pure_recover': "hn_invalid (pure Id) a1'a a1a
+      = hn_ctxt (pure Id) a1'a a1a * true"
+  unfolding hn_ctxt_def by(simp add: invalid_pure_recover)
 
 schematic_goal rd_hnr:
- "hn_refine emp ?C ?G ?R (rd_impl1 as)" using [[goals_limit = 1]]
+  "hn_refine emp (?C::?'a Heap) ?G ?R (rd_impl1 as)" using [[goals_limit = 3]]
   unfolding rd_impl1_def
   apply(rule hnr_bind)
-    apply(rule hnr_uRETURN_pure[where R=Id]) 
+    focus (* line 1 *)
+      apply(rule hnr_uRETURN_pure[where R=Id]) 
       apply simp
-
-   apply(rule hnr_bind) apply simp
-   apply(rule hnr_frame)
+    solved
+ 
+  apply(rule hnr_bind)
+    focus (* line 2 *) 
+      apply simp
+      apply(rule hnr_frame)
       apply(rule set_init_hnr')
 
      apply(simp add: entailst_def) apply(rule match_rest) apply simp
-
+    solved
   
   apply(rule hnr_bind)
+    focus (* line 3 *)
       apply(rule hnr_frame[OF hnr_uRETURN_pure[where R=Id]]) apply simp
-  apply(simp) apply(rule entt_refl)
-
+      apply(simp) apply(rule entt_refl)
+    solved
 
   apply(rule hnr_bind)
-
-  unfolding whileT_I' unfolding WHILEIT_to_monadic     
+    focus (* the while loop *)
+    unfolding whileT_I' unfolding WHILEIT_to_monadic     
 (*      apply(rule hn_monadic_WHILE_aux[where Rs="\<lambda>(c1,c2,c3) (a1,a2,a3). (pure Id) c1 a1 * (pure Id) c2 a2 * rbt_map_assn' c3 a3"])
   unfolding entailst_def
           apply rotatel apply(rule match_first)
@@ -359,55 +403,144 @@ schematic_goal rd_hnr:
           apply(rule hn_ctxt_triple')
   unfolding hn_ctxt_triple''
  *) 
-     apply(rule hn_monadic_WHILE_aux[where Rs="pure (Id) \<times>\<^sub>a  (pure (Id) \<times>\<^sub>a  rbt_map_assn')"])
+    apply(rule hn_monadic_WHILE_aux[where \<Gamma>="emp" and Rs="pure (Id) \<times>\<^sub>a  (pure (Id) \<times>\<^sub>a  rbt_map_assn')"])
+    focus (* WHILE: precondition *)
   unfolding entailst_def apply(simp  )
-           apply(rule ent_true_drop(2)) apply(rotater)
-          apply(rule ent_true_drop(2))
+           apply(rule ent_true_drop(2))  
            apply(subst hn_ctxt_prod_split'') prefer 2
             apply(subst hn_ctxt_prod_split'') prefer 2
-             apply rotater apply(rule match_first)  apply(rule match_first)  apply(rule entails_triv) apply simp
-           apply simp
-    (* loop guard *)
-  defer 
-  apply(rule match_rest) apply simp
+      apply rotater apply(rule match_first)  apply(rule match_first)  apply(rule entails_triv)
+      apply (rule refl) apply (rule refl)
+    solved
+    focus  (* WHILE: loop guard *)
+      unfolding b
+      (* split case_prod *)
+      apply(rule hn_case_prod')
+      focus (* 1st prod frame *)
+           unfolding entailst_def  apply rotatel apply(rule match_first)
+          apply(rule match_rest) apply simp
+      solved
+      apply(rule hn_refine_cons_post')
+      apply(rule hn_case_prod')
+      focus (* 2nd prod frame *)
+      unfolding entailst_def  apply rotatel apply(rule match_first)
+           apply(rule match_rest) apply simp
+      solved 
+      (* While: guard: code *)
+       focus
 
-   (* the loop body *)
-   apply(rule hn_case_prod')        
-    apply(simp add: entailst_def  )
+      apply(rule hnr_bind) (* bind Wg1 *)
+      focus (* While: guard: first return *)
+      apply(rule hnr_frame[OF hnr_uRETURN_pure[where R=Id]])
+       apply simp
+      unfolding entailst_def apply rotater apply rotatel apply rotatel apply (rule match_first)
+      apply rotater 
+           apply(rule ent_true_drop(2)) 
+      apply(rule entails_triv)
+      solved
+
+      apply(rule hnr_bind) (* bind Wg2 *)
+      focus (* While: guard: second return *)
+      apply(rule hnr_frame[OF hn_refine_length])
+        apply simp apply (simp add: entailst_def)
+      apply(rule ent_true_drop(2)) 
+      apply rotatel apply rotater apply(rule match_first)
+      apply (rule entails_triv)
+      solved
+      
+      focus (* While: guard: less *)
+      apply(rule hnr_frame[OF hn_refine_less])
+  apply (simp add: entailst_def)
+      apply(rule ent_true_drop(2)) 
+      apply rotater apply rotatel apply rotatel apply rotatel apply rotatel apply rotatel apply rotatel
+      apply (rule match_first)  apply rotatel  apply rotatel  apply rotatel
+      apply (rule match_first)
+      apply (rule entails_triv)
+      solved
+      
+      focus (* IMP of bind Wg2 *)
+        apply (simp add: entailst_def)   
+      apply(rule ent_true_drop(2)) 
+      apply rotater   apply rotatel      apply rotatel apply rotatel apply rotatel                  
+      apply rotatel     apply(rule match_first) apply(rule entails_triv)
+      solved
+
+      focus (* IMP of bind Wg1 *)
+      apply rotater  apply rotater apply rotater  apply rotater
+      apply (rule match_first) apply rotatel apply rotatel
+      apply rotater apply rotater apply rotater apply (rule match_first)
+      apply rotater apply rotater  apply (rule match_first)
+      apply(rule addemp_triv)
+      apply rotatel apply (rule match_first)
+      apply(rule ent_true_drop(2)) apply simp apply (rule entails_triv)
+      solved
+      solved 
+
+      apply rotatel apply rotatel apply (rule match_first) apply (rule match_first)
+      apply (rule match_rest)  
+      apply(rule ent_true_drop(2)) apply (rule entails_triv)
+      solved (* WHILE: loop guard *)
+
+      focus (* While : guard frame *)
+      apply(simp add: entailst_def)
+      apply(rule ent_true_drop(2))  
+      apply(rule entails_triv)
+      solved
+  
+
+   focus (* WHILE: the loop body *)
+      apply(rule hn_case_prod')     
+      focus (* 1st prod frame *)
+          unfolding entailst_def
           apply rotatel apply(rule match_first) apply(rule match_rest) apply simp
+      solved
+          apply(rule hn_refine_cons_post')
+          focus (* post R *)
+          apply(rule hn_case_prod')  
+      focus (* 2nd prod frame *)
+          unfolding entailst_def
+          apply rotatel  apply (rule match_first) apply(rule ent_true_drop_fst) apply(rule ent_true_drop(2))
+          apply (rule entails_triv) 
+      solved 
+      focus (* code *)   
+        apply(rule hnr_ASSERT)
+        apply(rule hnr_ASSERT)
+        apply(rule hnr_ASSERT) 
 
-         apply(rule hn_refine_cons_post'[OF hn_case_prod'])
-           apply(simp add: entailst_def  )
-           apply rotatel  apply (rule match_first)
-  apply rotater apply (rule match_first) apply (rule entails_triv) 
-         
-  apply(rule hnr_ASSERT)
-  apply(rule hnr_ASSERT)
-          apply(rule hnr_ASSERT) 
-  (* the hd operation *)
-  apply(rule hnr_bind[where Rh="pure Id"]) 
+       apply(rule hnr_bind[where Rh="pure Id"])  (* bind Wb1 *)
+      focus (* the hd operation *)
           apply(rule hnr_frame[OF hn_refine_hd])   
             apply(simp add: entailst_def) apply rotatel apply rotatel apply rotatel apply rotater apply (rule match_first)
   apply rotater 
             apply(rule ent_true_drop(2)) apply (rule entails_triv)
-  (* the tl operation *)
-  apply(rule hnr_bind[where Rh="pure Id"]) 
+     solved (* the hd operation *)
+
+     focus (* prog after hd *)
+       apply(rule hnr_bind[where Rh="pure Id"])  (* bind Wb2 *)
+      focus (* the tl operation *)
           apply(rule hnr_frame[OF hn_refine_tl])   
              apply(simp add: entailst_def mult.assoc) apply rotater apply rotatel apply rotatel    apply rotatel  apply rotatel
                 apply (rule match_first)
   apply rotater 
             apply(rule ent_true_drop(2)) apply (rule entails_triv)
-  (* the \<in> operation *)
-  apply(rule hnr_bind )              
-  apply(rule hnr_frame)
+      solved (* the tl operation *)
+
+     focus (* prog after tl *)
+    apply(rule hnr_bind )     (* bind Wb3 *)
+    focus (* the \<in> operation *)
+      apply(rule hnr_frame)
                apply(rule set_mem_hnr') 
-  apply(simp add: entailst_def)
+        apply(simp add: entailst_def)
             apply(rule ent_true_drop(2)) 
               apply rotater   apply rotatel apply rotatel apply rotatel
-              apply(rule isolate_first) apply(simp add: hn_ctxt_def) apply(rule entails_triv)
+          apply(rule isolate_first) apply(simp add: hn_ctxt_def) apply(rule entails_triv)
+             apply rotatel apply rotatel apply rotatel
+          apply(rule match_first)
               apply (rule entails_triv)
+      solved (* the \<in> operation *)
 
-  (* the if Block *)
+     focus (* prog after \<in> *)
+      focus (* the if Block *)
              apply(rule hnr_If')
                 apply rotater apply rotatel apply rotatel apply rotatel apply rotatel apply rotatel apply rotatel apply rotatel
                 apply(rule isolate_first)
@@ -417,28 +550,29 @@ schematic_goal rd_hnr:
             apply(rule ent_true_drop(2)) 
                 apply (rule entails_triv)
 
-  (* 1st if-branch (element already in list ) *)
+      focus (* 1st if-branch (element already in list ) *)
                apply(rule hnr_frame) 
                 apply(rule hnr_uRETURN_pass)
 
   
                apply(simp add: entailst_def)
-  apply rotater apply rotatel apply rotatel apply swapl apply swapl
+  apply rotater apply rotatel apply swapl apply swapl
   apply swapl apply swapl  apply swapl apply swapl  
                apply swapl apply swapl  apply swapl apply takel apply takel 
   apply(rule isolate_first)
                 apply(simp add:  gr_def     ) 
                 apply(subst hn_ctxt_prod_split'') prefer 2
-  apply(simp add: mult.assoc)
+  apply(simp add: mult.assoc) apply rotatel
   apply(rule match_first)
-                apply(subst hn_ctxt_prod_split'') prefer 2
+                apply(subst hn_ctxt_prod_split'') prefer 2 apply rotatel
   apply(rule match_first) apply(simp add: hn_ctxt_def) apply(rule entails_triv)
   apply simp apply simp
   apply rotater 
             apply(rule ent_true_drop(2)) 
                 apply (rule entails_triv)
+      solved (* 1st if-branch *)
 
-  (* 2nd if-branch (element should be added ) *)
+      focus  (* 2nd if-branch (element should be added ) *)
 
   apply (rule hnr_bind)
   (* \<rightarrow> add element into Set *)
@@ -446,8 +580,9 @@ schematic_goal rd_hnr:
   apply(rule set_ins_hnr')
                 apply(simp add: entailst_def)
             apply(rule ent_true_drop(2)) 
-                apply rotater apply rotatel apply rotatel apply rotatel apply rotatel apply rotatel apply rotatel
-  apply(rule match_first) 
+                apply rotater apply rotatel apply rotatel apply rotatel apply rotatel apply rotatel
+            apply(rule match_first) 
+                apply(rule match_first) 
                 apply (rule entails_triv)
 
                apply (rule hnr_bind)
@@ -458,9 +593,9 @@ schematic_goal rd_hnr:
   apply(rule hnr_cons_rule)
                 apply(simp add: entailst_def)
             apply(rule ent_true_drop(2)) 
-                 apply rotater apply taker apply rotatel apply rotatel apply rotatel
-                 apply rotatel apply swapl apply takel apply (rule isolate_first)
-                  apply(simp add: gr_def) apply rotatel apply (rule match_first)
+                 apply rotater apply taker apply rotatel apply rotatel apply swapl apply swapl
+                 apply swapl  apply takel apply (rule isolate_first)
+                  apply(simp add: gr_def)  apply (rule match_first)
                   apply (rule entails_triv) apply(rule entails_triv)
 
   (* \<rightarrow> return result *)
@@ -469,13 +604,13 @@ schematic_goal rd_hnr:
 
                apply(simp add: entailst_def)
             apply(rule ent_true_drop(2)) 
-                apply rotater apply rotatel apply rotatel apply rotatel apply rotatel
-                apply swapl apply swapl apply swapl apply takel apply takel
+                apply rotater apply rotatel apply rotatel apply rotatel apply rotatel apply rotatel
+                apply swapl   apply swapl apply takel apply takel
                 apply (rule isolate_first)
   apply(simp only: gr_def)
                 apply(subst hn_ctxt_prod_split'') prefer 2
   apply(simp add: mult.assoc)
-  apply(rule match_first)
+  apply(rule match_first)  
                 apply(subst hn_ctxt_prod_split'') prefer 2
   apply(rule match_first) apply(simp add: hn_ctxt_def) apply(rule entails_triv)
   apply simp apply simp
@@ -494,19 +629,22 @@ schematic_goal rd_hnr:
             apply(rule ent_true_drop(2)) 
   apply rotater               
                apply(rule match_first) 
-               apply(rule entails_triv)      
+      apply(rule entails_triv) 
+      solved (* 2nd if-branch *)
 
             apply(rule ent_true_drop(2)) 
              apply(rule entails_triv)
+  solved (* the if Block *)
+  solved (* prog after \<in> *)
 
-  (* merge the heap or *)
-  apply(simp only: mult.assoc)
+  focus (* IMP of bind Wb3: merge the heap or *)
+          unfolding mult.assoc
             apply(rule addemp_triv)
+            apply(rule ent_trans[OF or_merge_rotatel])
+  apply(simp only: mult.assoc) 
             apply(rule ent_trans[OF or_merge_succ_step]) 
             apply(rule ent_trans[OF or_merge_succ_step]) 
-            apply(rule ent_trans[OF or_merge_succ_step]) 
-            apply(rule ent_trans[OF or_merge_rotatel]) 
-  apply(simp only: mult.assoc)
+            apply(rule ent_trans[OF or_merge_succ_step])  
             apply(rule ent_trans[OF or_merge_succ_step]) 
             apply(rule ent_trans[OF or_merge_rotatel]) 
             apply(rule ent_trans[OF or_merge_rotater]) 
@@ -524,31 +662,128 @@ schematic_goal rd_hnr:
             apply(rule ent_trans[OF or_merge_succ_step])
             apply(rule forward_ent_snd)
              apply(rule ent_trans) apply(rule underA[OF hn_invalid_prod_split])
-              apply(simp add: hn_ctxt_def invalid_pure_recover)
-  apply(rule or_merge)
-    
+              apply(simp add:   invalid_pure_recover')
+  apply(rule underB)
+              apply(rule addemp_triv) apply rotatel
+               apply(rule entails_triv) 
+  apply(simp only: mult.assoc)
+             apply(rule ent_trans[OF or_merge_succ_step]) 
+             apply(rule entails_triv)  
+
+            apply(rule forward_ent_snd)
+            apply(rule forward_ent_snd)
+              apply(rule entails_true)
+            apply(rule entails_triv)
 
             apply rotater
   apply(simp add: gr_def mult.assoc)
             apply(rule isolate_first)
              apply(simp add: hn_ctxt_def pure_def) apply(rule entails_triv)
   apply rotater
+  apply rotatel  apply rotatel  apply rotatel  apply rotatel  apply rotatel apply rotatel
+            apply(rule ent_true_drop_fst)
             apply(rule ent_true_drop(2))
             apply(rule entails_triv)
+  solved (* IMP of bind Wb3: merge the heap or *)
+  solved (* prog after tl *)
 
-  (* after *)
-   (* recover xd *) defer
-    
+  focus (* IMP of bind Wb2 *)
 
-               apply taker
-               apply(rule isolate_first)
-  apply(simp only: hn_ctxt_def gr_def invalid_pure_recover)
-                apply(rule match_first) apply simp
-                apply (rule entails_triv)
-              apply(simp add: mult.assoc)
+  (* after *) 
+  apply rotater apply rotatel apply rotatel apply rotatel apply rotatel 
+  apply(rule match_first) 
   apply rotater 
+            apply(rule ent_true_drop(2))
+           apply(rule entails_triv)
+  solved (* IMP of bind Wb2 *)
+  solved (* prog after hd *)                                
 
+          focus (* IMP of bind Wb1 *)
+          unfolding mult.assoc
+            apply(rule match_first)
+              apply rotater 
+            apply(rule match_first) apply rotater   
+          apply rotatel apply rotatel apply(rule match_first)    
 
-  using hnr_cons_rule
+          apply(rule forward_ent[OF entails_true])
+          apply rotater apply(rule isolate_first)
+          apply(simp add: hn_ctxt_def) apply(rule entails_triv)
+ 
+            apply(rule ent_true_drop(2))
+          apply(rule entails_triv)
+          solved (* IMP of bind Wb1 *)
+          solved  (* code *)  
+          solved  (* post R *)
+          focus (* post I *)
+            apply rotater apply(rule match_first)
+            apply rotater apply rotater apply rotater
+              apply(rule addemp_triv) apply rotatel apply(rule match_first)
+            apply(rule addemp_triv) apply(rule isolate_first)
+            apply(simp add: hn_ctxt_def) apply(rule entails_triv)
+              apply(rule ent_true_drop(2))
+            apply(rule entails_triv)
+          solved (* post I *)
+  solved  (* WHILE: the loop body *)
+          apply (simp add: entailst_def)
+          apply(rule ent_true_drop(2))
+          apply (simp add: hn_ctxt_def)
+          solved (* the while loop *)
+
+    
+   focus (* finally return result *)
+
+      (* split case_prod *)
+      apply(rule hn_case_prod')
+      focus (* 1st prod frame *)
+           unfolding entailst_def  apply rotatel apply rotatel apply(rule isolate_first)
+           apply(rule entails_triv)
+                  apply(rule match_rest) apply simp
+      solved
+      apply(rule hn_refine_cons_post')
+      apply(rule hn_case_prod')
+      focus (* 2nd prod frame *)
+      unfolding entailst_def  apply rotatel apply(rule match_first)
+           apply(rule match_rest) apply simp
+      solved 
+
+  
+      apply(rule hn_refine_cons_post')
+       apply(rule hnr_frame)  
+         apply(rule hnr_uRETURN_pass) unfolding entailst_def mult.assoc
+        apply rotater apply(rule isolate_first)  
+      (* shit happening here *)apply(rule entails_triv)  
+      apply rotater  apply(rule match_rest) apply simp
+
+      unfolding mult.assoc
+       apply rotater apply(rule match_first) 
+       apply rotatel apply rotatel apply rotatel apply rotatel apply (rule match_first)
+       apply rotater  apply rotater apply(rule match_first)
+       apply(rule match_rest) apply simp
+
+      apply rotater apply(rule match_first)
+      apply rotatel apply rotatel apply (rule match_first)
+      apply rotater apply rotater apply (rule match_first)
+      apply (rule match_rest) apply simp
+  solved (* finally return result *)
+
+      unfolding mult.assoc apply rotater apply (rule match_first)
+         apply rotater apply (rule match_rest) apply simp
+      apply rotatel
+      apply simp
+        apply(rule ent_trans[OF hn_invalid_prod_split])
+        apply rotater apply(rule match_first)
+        apply rotater apply(rule match_rest) apply simp
+
+       apply(rule ent_trans[OF hn_invalid_prod_split])
+       apply rotatel apply rotater apply (rule match_first)
+       apply rotater apply(rule match_rest) apply simp
+
+      apply rotater 
+      apply(rule addemp_triv)
+      apply rotatel apply(rule match_first)
+      apply rotater apply(rule match_rest) apply simp
+      solved 
+
+      done
 
 end
